code/ecdsap256/Hacl.Impl.P256.Signature.Common.fsti
@@ -19,18 +19,22 @@ open Hacl.Impl.P256.Core
 
 open FStar.Mul
 
+#set-options "--fuel 0 --ifuel 0 --z3rlimit 200"
 
 val bufferToJac: #c: curve -> p: lbuffer uint64 (getCoordinateLenU64 c *. 2ul) -> result: point c -> Stack unit
   (requires fun h -> live h p /\ live h result /\ disjoint p result)
   (ensures  fun h0 _ h1 ->
+    let len = getCoordinateLenU64 c in 
     modifies (loc result) h0 h1 /\
-    as_nat c h1 (gsub result (getCoordinateLenU64 c *. 2ul) (getCoordinateLenU64 c)) == 1 /\
+    as_nat c h1 (gsub result (len *. size 2) len) == 1 /\
     (
-      let x = as_nat c h0 (gsub p (size 0) (getCoordinateLenU64 c)) in
-      let y = as_nat c h0 (gsub p (getCoordinateLenU64 c) (getCoordinateLenU64 c)) in
+      let x = as_nat c h0 (gsub p (size 0) len) in
+      let y = as_nat c h0 (gsub p len len) in
       let x3, y3, z3 = point_x_as_nat c h1 result, point_y_as_nat c h1 result, point_z_as_nat c h1 result in
       let pointJacX, pointJacY, pointJacZ = toJacobianCoordinates (x, y) in
-      x3 == pointJacX /\ y3 == pointJacY /\ z3 == pointJacZ))
+      x3 == pointJacX /\ y3 == pointJacY /\ z3 == pointJacZ)
+      )
+
 
 
 [@ (Comment "  This code is not side channel resistant")]  
@@ -42,22 +46,25 @@ val isPointAtInfinityPublic: #c: curve -> p:point c -> Stack bool
 
 [@ (Comment "  This code is not side channel resistant")]
 val isPointOnCurvePublic: #c: curve -> p: point c -> Stack bool
-  (requires fun h -> live h p /\    
-    as_nat c h (gsub p (size 0) (size 4)) < prime256 /\ 
-    as_nat c h (gsub p (size 4) (size 4)) < prime256 /\
-    as_nat c h (gsub p (size 8) (size 4)) == 1)
+  (requires fun h -> 
+    let len = getCoordinateLenU64 c in 
+    let prime = getPrime c in 
+    live h p /\    
+    as_nat c h (gsub p (size 0) len) < prime /\ 
+    as_nat c h (gsub p len len) < prime /\
+    as_nat c h (gsub p (size 2 *! len) len) == 1)
   (ensures fun h0 r h1 ->
+    let len = getCoordinateLenU64 c in 
     modifies0 h0 h1 /\ 
-     r == isPointOnCurve #P256 (as_nat c h1 (gsub p (size 0) (size 4)), 
-                          as_nat c h1 (gsub p (size 4) (size 4)), 
-                          as_nat c h1 (gsub p (size 8) (size 4)))
+    r == isPointOnCurve #c (as_nat c h1 (gsub p (size 0) len), 
+                          as_nat c h1 (gsub p len len), 
+                          as_nat c h1 (gsub p (size 2 *! len) len))
   )
 
 
-(* [@ (Comment "  This code is not side channel resistant")] *)
-
+[@ (Comment "  This code is not side channel resistant")] 
 val verifyQValidCurvePoint: #c: curve -> pubKeyAsPoint: point c
-  -> tempBuffer:lbuffer uint64 (size 100) -> Stack bool
+  -> tempBuffer:lbuffer uint64 (size 25 *! getCoordinateLenU64 c) -> Stack bool
   (requires fun h ->
     live h pubKeyAsPoint /\
     live h tempBuffer /\
@@ -66,19 +73,19 @@ val verifyQValidCurvePoint: #c: curve -> pubKeyAsPoint: point c
   )
   (ensures  fun h0 r h1 ->
     modifies (loc tempBuffer) h0 h1 /\
-    r == verifyQValidCurvePointSpec #P256 (point_prime_to_coordinates c (as_seq h0 pubKeyAsPoint)))
+    r == verifyQValidCurvePointSpec #c (point_prime_to_coordinates c (as_seq h0 pubKeyAsPoint)))
 
 inline_for_extraction
 val verifyQ: 
   #c: curve ->
-  pubKey: lbuffer uint8 (size 64) ->
+  pubKey: lbuffer uint8 (size (getPointLen c)) ->
   Stack bool
     (requires fun h -> live h pubKey)
     (ensures  fun h0 r h1 -> modifies0 h0 h1 /\
       (
-	let publicKeyX = nat_from_bytes_be (as_seq h1 (gsub pubKey (size 0) (size 32))) in 
-	let publicKeyY = nat_from_bytes_be (as_seq h1 (gsub pubKey (size 32) (size 32))) in
+	let publicKeyX = nat_from_bytes_be (as_seq h1 (gsub pubKey (size 0) (size (getCoordinateLen c)))) in 
+	let publicKeyY = nat_from_bytes_be (as_seq h1 (gsub pubKey (size (getCoordinateLen c)) (size (getCoordinateLen c)))) in
 	let pkJ = Spec.P256.toJacobianCoordinates (publicKeyX, publicKeyY) in 
-	r == verifyQValidCurvePointSpec #P256 pkJ
+	r == verifyQValidCurvePointSpec #c pkJ
       )
     )
